src/HOL/CVC/cvc5_dsl_rewrites/Arith_Rewrites.thy
@@ -1,233 +1,259 @@
 theory Arith_Rewrites
-  imports Dsl_Nary_Ops "HOL.Real"
+  imports "HOL-CVC.Dsl_Nary_Ops" "Arith_Rewrites_Lemmas"
 begin
 
-(* This is a theory automatically created from a rare file! All that remains to do is to prove
-any lemma whose provided proof fails and to to import this file in SMT.thy. 
-If your rare statements use nary operators over lists that would be binarised by Isabelle 
-you have to add it in Dsl_Nary_Ops.thy. Currently already supported are the operators:
-and,
-or,
-plus,
-times,
-append,
-re_concat,
-str_concat,
-*)
+(* Thank you for using IsaRARE. This is a theory automatically created from a RARE file!
+All that remains to do is to prove any lemma whose provided proof fails.
+If you want to use the lemmas for proof reconstruction you'll also need to import this file in Rare_Interface.thy*)
 
 named_theorems rewrite_arith_plus_zero \<open>automatically_generated\<close>
 
 lemma [rewrite_arith_plus_zero]:
   fixes t::"int cvc_ListVar" and s::"int cvc_ListVar"
-  shows "NO_MATCH a (undefined t s) ==> cvc_list_right (+) (cvc_list_left (+) t (0::int)) s =
+  shows "NO_MATCH cvc_a (undefined t s) \<Longrightarrow> cvc_list_right (+) (cvc_list_left (+) t (0::int)) s =
    cvc_list_both (+) (0::int) t s"
   apply (cases s)
   apply (cases t)
   subgoal for ss ts 
     apply (simp add: cvc_list_left_transfer cvc_list_right_transfer_op cvc_list_both_transfer_op)
-    apply (induction ts arbitrary: t)
-    by simp_all
+    apply (induction ss)
+    apply simp_all
+    apply (induction ts)
+    apply simp_all
+    by (simp_all add: arith_plus_zero_lemma)
   done
+
 
 named_theorems rewrite_arith_mul_one \<open>automatically_generated\<close>
 
 lemma [rewrite_arith_mul_one]:
   fixes t::"int cvc_ListVar" and s::"int cvc_ListVar"
-  shows "NO_MATCH a (undefined t s) ==> cvc_list_right (*) (cvc_list_left (*) t (1::int)) s =
+  shows "NO_MATCH cvc_a (undefined t s) \<Longrightarrow> cvc_list_right (*) (cvc_list_left (*) t (1::int)) s =
    cvc_list_both (*) (1::int) t s"
   apply (cases s)
   apply (cases t)
   subgoal for ss ts 
     apply (simp add: cvc_list_left_transfer cvc_list_right_transfer_op cvc_list_both_transfer_op)
-    apply (induction ts arbitrary: t)
-    by simp_all
+    apply (induction ss)
+    apply simp_all
+    apply (induction ts)
+    apply simp_all
+    by (simp_all add: arith_mul_one_lemma)
   done
+
 
 named_theorems rewrite_arith_mul_zero \<open>automatically_generated\<close>
 
 lemma [rewrite_arith_mul_zero]:
   fixes t::"int cvc_ListVar" and s::"int cvc_ListVar"
-  shows "NO_MATCH a (undefined t s) ==> cvc_list_right (*) (cvc_list_left (*) t (0::int)) s = (0::int)"
+  shows "NO_MATCH cvc_a (undefined t s) \<Longrightarrow> cvc_list_right (*) (cvc_list_left (*) t (0::int)) s = (0::int)"
   apply (cases s)
   apply (cases t)
   subgoal for ss ts 
     apply (simp add: cvc_list_left_transfer cvc_list_right_transfer_op cvc_list_both_transfer_op)
-    apply (induction ts arbitrary: t)
-    by simp_all
+    apply (induction ss)
+    apply simp_all
+    apply (induction ts)
+    apply simp_all
+    by (simp_all add: arith_mul_zero_lemma)
   done
+
+
+named_theorems rewrite_arith_int_div_one \<open>automatically_generated\<close>
+
+lemma [rewrite_arith_int_div_one]:
+  fixes t::"int"
+  shows "NO_MATCH cvc_a (undefined t) \<Longrightarrow> SMT.z3div t (1::int) = t"
+  by (simp add: SMT.z3div_def)
+
 
 named_theorems rewrite_arith_neg_neg_one \<open>automatically_generated\<close>
 
 lemma [rewrite_arith_neg_neg_one]:
-  fixes t::"nat"
-  shows "NO_MATCH a (undefined t) ==> - (1::int) * (- (1::int) * t) = t"
+  fixes t::"int"
+  shows "NO_MATCH cvc_a (undefined t) \<Longrightarrow> - (1::int) * (- (1::int) * t) = t"
   by auto
+
 
 named_theorems rewrite_arith_elim_uminus \<open>automatically_generated\<close>
 
 lemma [rewrite_arith_elim_uminus]:
   fixes t::"int"
-  shows "NO_MATCH a (undefined t) ==> - t = - (1::int) * t"
+  shows "NO_MATCH cvc_a (undefined t) \<Longrightarrow> - t = - (1::int) * t"
   by auto
+
 
 named_theorems rewrite_arith_elim_minus \<open>automatically_generated\<close>
 
 lemma [rewrite_arith_elim_minus]:
   fixes t::"int" and s::"int"
-  shows "NO_MATCH a (undefined t s) ==> t - s = t + - (1::int) * s"
+  shows "NO_MATCH cvc_a (undefined t s) \<Longrightarrow> t - s = t + - (1::int) * s"
   by auto
+
 
 named_theorems rewrite_arith_elim_gt \<open>automatically_generated\<close>
 
 lemma [rewrite_arith_elim_gt]:
   fixes t::"'a::linorder" and s::"'a::linorder"
-  shows "NO_MATCH a (undefined t s)==> (s < t) = (\<not> t \<le> s)"
-  using linorder_not_less by blast
+  shows "NO_MATCH cvc_a (undefined t s) \<Longrightarrow> (s < t) = (\<not> t \<le> s)"
+  by auto
+
 
 named_theorems rewrite_arith_elim_lt \<open>automatically_generated\<close>
 
 lemma [rewrite_arith_elim_lt]:
   fixes t::"'a::linorder" and s::"'a::linorder"
-  shows "NO_MATCH a (undefined t s) ==> (t < s) = (\<not> s \<le> t)"
-    using linorder_not_less by blast
+  shows "NO_MATCH cvc_a (undefined t s) \<Longrightarrow> (t < s) = (\<not> s \<le> t)"
+  by auto
 
 
 named_theorems rewrite_arith_elim_leq \<open>automatically_generated\<close>
 
 lemma [rewrite_arith_elim_leq]:
-  fixes t::"'a::ord" and s::"'a::ord"
-  shows "NO_MATCH a (undefined t s) ==> (t \<le> s) = (t \<le> s)"
+  fixes t::"'a::linorder" and s::"'a::linorder"
+  shows "NO_MATCH cvc_a (undefined t s) \<Longrightarrow> (t \<le> s) = (t \<le> s)"
   by auto
+
 
 named_theorems rewrite_arith_leq_norm \<open>automatically_generated\<close>
 
 lemma [rewrite_arith_leq_norm]:
   fixes t::"int" and s::"int"
-  shows "NO_MATCH a (undefined t s) ==> (t \<le> s) = (\<not> s + (1::int) \<le> t)"
+  shows "NO_MATCH cvc_a (undefined t s) \<Longrightarrow> (t \<le> s) = (\<not> s + (1::int) \<le> t)"
   by auto
+
 
 named_theorems rewrite_arith_geq_tighten \<open>automatically_generated\<close>
 
 lemma [rewrite_arith_geq_tighten]:
   fixes t::"int" and s::"int"
-  shows "NO_MATCH a (undefined t s)  ==> (\<not> s \<le> t) = (t + (1::int) \<le> s)"
+  shows "NO_MATCH cvc_a (undefined t s) \<Longrightarrow> (\<not> s \<le> t) = (t + (1::int) \<le> s)"
   by auto
+
 
 named_theorems rewrite_arith_geq_norm \<open>automatically_generated\<close>
 
 lemma [rewrite_arith_geq_norm]:
   fixes t::"int" and s::"int"
-  shows "NO_MATCH a (undefined t s) ==> (s \<le> t) = ((0::int) \<le> t - s)"
+  shows "NO_MATCH cvc_a (undefined t s) \<Longrightarrow> (s \<le> t) = ((0::int) \<le> t - s)"
   by auto
+
 
 named_theorems rewrite_arith_refl_leq \<open>automatically_generated\<close>
 
 lemma [rewrite_arith_refl_leq]:
   fixes t::"'a::linorder"
-  shows "NO_MATCH a (undefined t) ==> (t \<le> t) = True"
+  shows "NO_MATCH cvc_a (undefined t) \<Longrightarrow> (t \<le> t) = True"
   by auto
+
 
 named_theorems rewrite_arith_refl_lt \<open>automatically_generated\<close>
 
 lemma [rewrite_arith_refl_lt]:
   fixes t::"'a::linorder"
-  shows "NO_MATCH a (undefined t) ==> (t < t) = False"
+  shows "NO_MATCH cvc_a (undefined t) \<Longrightarrow> (t < t) = False"
   by auto
+
 
 named_theorems rewrite_arith_refl_geq \<open>automatically_generated\<close>
 
 lemma [rewrite_arith_refl_geq]:
   fixes t::"'a::linorder"
-  shows "NO_MATCH a (undefined t) ==> (t \<le> t) = True"
+  shows "NO_MATCH cvc_a (undefined t) \<Longrightarrow> (t \<le> t) = True"
   by auto
+
 
 named_theorems rewrite_arith_refl_gt \<open>automatically_generated\<close>
 
 lemma [rewrite_arith_refl_gt]:
   fixes t::"'a::linorder"
-  shows "NO_MATCH a (undefined t) ==> (t < t) = False"
+  shows "NO_MATCH cvc_a (undefined t) \<Longrightarrow> (t < t) = False"
   by auto
+
 
 named_theorems rewrite_arith_plus_flatten \<open>automatically_generated\<close>
 
 lemma [rewrite_arith_plus_flatten]:
-  fixes xs::"'a::linordered_ab_group_add cvc_ListVar" and w::"'a::linordered_ab_group_add" and ys::"'a::linordered_ab_group_add cvc_ListVar" and zs::"'a::linordered_ab_group_add cvc_ListVar"
-  shows "NO_MATCH a (undefined xs w ys zs) ==> cvc_list_right (+) (cvc_list_left (+) xs (cvc_list_right (+) w ys)) zs =
+  fixes xs::"int cvc_ListVar" and w::"int" and ys::"int cvc_ListVar" and zs::"int cvc_ListVar"
+  shows "NO_MATCH cvc_a (undefined xs w ys zs) \<Longrightarrow> cvc_list_right (+) (cvc_list_left (+) xs (cvc_list_right (+) w ys)) zs =
    cvc_list_right (+) (cvc_list_right (+) (cvc_list_left (+) xs w) ys) zs"
   apply (cases zs)
   apply (cases ys)
   apply (cases xs)
   subgoal for zss yss xss 
     apply (simp add: cvc_list_left_transfer cvc_list_right_transfer_op cvc_list_both_transfer_op)
-    apply (induction xss arbitrary: xs)
-    by simp_all
+    apply (induction zss)
+    apply simp_all
+    apply (induction yss)
+    apply simp_all
+    apply (induction xss)
+    apply simp_all
+    by (simp_all add: arith_plus_flatten_lemma)
   done
+
 
 named_theorems rewrite_arith_mult_flatten \<open>automatically_generated\<close>
 
 lemma [rewrite_arith_mult_flatten]:
-  fixes xs::"'a::ab_semigroup_mult cvc_ListVar" and w::"'a::ab_semigroup_mult" and ys::"'a::ab_semigroup_mult cvc_ListVar" and zs::"'a::ab_semigroup_mult cvc_ListVar"
-  shows "NO_MATCH a (undefined xs w ys zs) ==> cvc_list_right (*) (cvc_list_left (*) xs (cvc_list_right (*) w ys)) zs =
+  fixes xs::"int cvc_ListVar" and w::"int" and ys::"int cvc_ListVar" and zs::"int cvc_ListVar"
+  shows "NO_MATCH cvc_a (undefined xs w ys zs) \<Longrightarrow> cvc_list_right (*) (cvc_list_left (*) xs (cvc_list_right (*) w ys)) zs =
    cvc_list_right (*) (cvc_list_right (*) (cvc_list_left (*) xs w) ys) zs"
   apply (cases zs)
   apply (cases ys)
   apply (cases xs)
   subgoal for zss yss xss 
     apply (simp add: cvc_list_left_transfer cvc_list_right_transfer_op cvc_list_both_transfer_op)
-    apply (induction xss arbitrary: xs)
-     apply simp_all
-    apply (induction yss arbitrary: ys)
-     apply simp_all
-    apply (simp add: cvc_list_right_Nil)
-     apply (induction zss arbitrary: zs)
-    apply (simp add: cvc_list_right_Nil cvc_list_right_transfer mult.assoc)
-     apply (simp add: ab_semigroup_mult_class.mult_ac(1) cvc_list_right_Cons)
-    by (simp add: cvc_list_right_Cons mult.assoc)
+    apply (induction zss)
+    apply simp_all
+    apply (induction yss)
+    apply simp_all
+    apply (induction xss)
+    apply simp_all
+    by (simp_all add: arith_mult_flatten_lemma)
   done
+
 
 named_theorems rewrite_arith_mult_dist \<open>automatically_generated\<close>
 
 lemma [rewrite_arith_mult_dist]:
-  fixes x::"'a::{ring}" and y::"'a" and z::"'a" and w::"'a cvc_ListVar"
-  shows "NO_MATCH a (undefined x y z w) ==> x * cvc_list_right (+) (y + z) w = x * y + x * cvc_list_right (+) z w"
+  fixes x::"int" and y::"int" and z::"int" and w::"int cvc_ListVar"
+  shows "NO_MATCH cvc_a (undefined x y z w) \<Longrightarrow> x * cvc_list_right (+) (y + z) w = x * y + x * cvc_list_right (+) z w"
   apply (cases w)
   subgoal for ws 
     apply (simp add: cvc_list_left_transfer cvc_list_right_transfer_op cvc_list_both_transfer_op)
-    apply (induction ws arbitrary: w)
-     apply simp_all
-    unfolding cvc_list_right_def
-     apply (simp add: ring_class.ring_distribs(1))
-    by (simp add: ring_class.ring_distribs(1))
+    apply (induction ws)
+    apply simp_all
+    by (simp_all add: arith_mult_dist_lemma)
   done
+
 
 named_theorems rewrite_arith_plus_cancel1 \<open>automatically_generated\<close>
 
 lemma [rewrite_arith_plus_cancel1]:
-  fixes t::"('a::{zero,plus,one,times,uminus}) cvc_ListVar" and x::"'a::{zero,plus,one,times,uminus}" and s::"'a::{zero,plus,one,times,uminus} cvc_ListVar" 
-and r::"'a::{zero,plus,one,times,uminus} cvc_ListVar"
-  shows "NO_MATCH a (undefined t x s r) ==> cvc_list_right (+)
-    (cvc_list_right (+) (cvc_list_left (+) t x) s + - 1 * x) r =
-   cvc_list_right (+) (cvc_list_both (+) 0 t s) r"
+  fixes t::"int cvc_ListVar" and x::"int" and s::"int cvc_ListVar" and r::"int cvc_ListVar"
+  shows "NO_MATCH cvc_a (undefined t x s r) \<Longrightarrow> cvc_list_right (+)
+    (cvc_list_right (+) (cvc_list_left (+) t x) s + - (1::int) * x) r =
+   cvc_list_right (+) (cvc_list_both (+) (0::int) t s) r"
   apply (cases r)
   apply (cases s)
   apply (cases t)
   subgoal for rs ss ts 
     apply (simp add: cvc_list_left_transfer cvc_list_right_transfer_op cvc_list_both_transfer_op)
     apply (induction rs)
-     apply simp_all
-    apply (induction ts)
-     apply simp_all
+    apply simp_all
     apply (induction ss)
-     apply simp_all
-    
-    sorry
+    apply simp_all
+    apply (induction ts)
+    apply simp_all
+    by (simp_all add: arith_plus_cancel1_lemma)
   done
+
 
 named_theorems rewrite_arith_plus_cancel2 \<open>automatically_generated\<close>
 
 lemma [rewrite_arith_plus_cancel2]:
   fixes t::"int cvc_ListVar" and x::"int" and s::"int cvc_ListVar" and r::"int cvc_ListVar"
-  shows "NO_MATCH a (undefined t x s r) ==> cvc_list_right (+)
+  shows "NO_MATCH cvc_a (undefined t x s r) \<Longrightarrow> cvc_list_right (+)
     (cvc_list_right (+) (cvc_list_left (+) t (- (1::int) * x)) s + x) r =
    cvc_list_right (+) (cvc_list_both (+) (0::int) t s) r"
   apply (cases r)
@@ -235,7 +261,13 @@ lemma [rewrite_arith_plus_cancel2]:
   apply (cases t)
   subgoal for rs ss ts 
     apply (simp add: cvc_list_left_transfer cvc_list_right_transfer_op cvc_list_both_transfer_op)
-    sorry
+    apply (induction rs)
+    apply simp_all
+    apply (induction ss)
+    apply simp_all
+    apply (induction ts)
+    apply simp_all
+    by (simp_all add: arith_plus_cancel2_lemma)
   done
 
 end
