src/HOL/CVC/cvc5_dsl_rewrites/Boolean_Rewrites.thy
@@ -1,90 +1,100 @@
 theory Boolean_Rewrites
-  imports Dsl_Nary_Ops Boolean_Rewrites_Lemmas
+  imports "HOL-CVC.Dsl_Nary_Ops" "Boolean_Rewrites_Lemmas"
 begin
 
-(* This is a theory automatically created from a RARE file! All that remains to do is to prove
-any lemma whose provided proof fails and to to import this file in SMT.thy (if you want to use it
-for proof reconstruction).*)
+(* Thank you for using IsaRARE. This is a theory automatically created from a RARE file!
+All that remains to do is to prove any lemma whose provided proof fails.
+If you want to use the lemmas for proof reconstruction you'll also need to import this file in Rare_Interface.thy*)
 
 named_theorems rewrite_bool_double_not_elim \<open>automatically_generated\<close>
 
 lemma [rewrite_bool_double_not_elim]:
   fixes t::"bool"
-  shows "NO_MATCH a (undefined t) ==> (\<not> \<not> t) = t"
+  shows "NO_MATCH cvc_a (undefined t) \<Longrightarrow> (\<not> \<not> t) = t"
   by auto
+
 
 named_theorems rewrite_bool_eq_true \<open>automatically_generated\<close>
 
 lemma [rewrite_bool_eq_true]:
   fixes t::"bool"
-  shows "NO_MATCH a (undefined t) ==> (t = True) = t"
+  shows "NO_MATCH cvc_a (undefined t) \<Longrightarrow> (t = True) = t"
   by auto
+
 
 named_theorems rewrite_bool_eq_false \<open>automatically_generated\<close>
 
 lemma [rewrite_bool_eq_false]:
   fixes t::"bool"
-  shows "NO_MATCH a (undefined t) ==> (t = False) = (\<not> t)"
+  shows "NO_MATCH cvc_a (undefined t) \<Longrightarrow> (t = False) = (\<not> t)"
   by auto
+
 
 named_theorems rewrite_bool_eq_nrefl \<open>automatically_generated\<close>
 
 lemma [rewrite_bool_eq_nrefl]:
   fixes x::"bool"
-  shows "NO_MATCH a (undefined x) ==> (x = (\<not> x)) = False"
+  shows "NO_MATCH cvc_a (undefined x) \<Longrightarrow> (x = (\<not> x)) = False"
   by auto
+
 
 named_theorems rewrite_bool_impl_false1 \<open>automatically_generated\<close>
 
 lemma [rewrite_bool_impl_false1]:
   fixes t::"bool"
-  shows "NO_MATCH a (undefined t) ==> (t \<longrightarrow> False) = (\<not> t)"
+  shows "NO_MATCH cvc_a (undefined t) \<Longrightarrow> (t \<longrightarrow> False) = (\<not> t)"
   by auto
+
 
 named_theorems rewrite_bool_impl_false2 \<open>automatically_generated\<close>
 
 lemma [rewrite_bool_impl_false2]:
   fixes t::"bool"
-  shows "NO_MATCH a (undefined t) ==> (False \<longrightarrow> t) = True"
+  shows "NO_MATCH cvc_a (undefined t) \<Longrightarrow> (False \<longrightarrow> t) = True"
   by auto
+
 
 named_theorems rewrite_bool_impl_true1 \<open>automatically_generated\<close>
 
 lemma [rewrite_bool_impl_true1]:
   fixes t::"bool"
-  shows "NO_MATCH a (undefined t) ==> (t \<longrightarrow> True) = True"
+  shows "NO_MATCH cvc_a (undefined t) \<Longrightarrow> (t \<longrightarrow> True) = True"
   by auto
+
 
 named_theorems rewrite_bool_impl_true2 \<open>automatically_generated\<close>
 
 lemma [rewrite_bool_impl_true2]:
   fixes t::"bool"
-  shows "NO_MATCH a (undefined t) ==> (True \<longrightarrow> t) = t"
+  shows "NO_MATCH cvc_a (undefined t) \<Longrightarrow> (True \<longrightarrow> t) = t"
   by auto
+
 
 named_theorems rewrite_bool_impl_elim \<open>automatically_generated\<close>
 
 lemma [rewrite_bool_impl_elim]:
   fixes t::"bool" and s::"bool"
-  shows "(t \<longrightarrow> s) = (\<not> t \<or> s)"
+  shows "NO_MATCH cvc_a (undefined t s) \<Longrightarrow> (t \<longrightarrow> s) = (\<not> t \<or> s)"
   by auto
+
 
 named_theorems rewrite_bool_or_true \<open>automatically_generated\<close>
 
 lemma [rewrite_bool_or_true]:
   fixes xs::"bool cvc_ListVar" and ys::"bool cvc_ListVar"
-  shows "NO_MATCH a (undefined xs ys) ==> cvc_list_left (\<or>) xs (cvc_list_right (\<or>) True ys) = True"
+  shows "NO_MATCH cvc_a (undefined xs ys) \<Longrightarrow> cvc_list_left (\<or>) xs (cvc_list_right (\<or>) True ys) = True"
   apply (cases ys)
   apply (cases xs)
   subgoal for yss xss 
     by (simp add: cvc_list_left_transfer cvc_list_right_transfer_op cvc_list_both_transfer_op)
   done
 
+
 named_theorems rewrite_bool_or_false \<open>automatically_generated\<close>
 
 lemma [rewrite_bool_or_false]:
   fixes xs::"bool cvc_ListVar" and ys::"bool cvc_ListVar"
-  shows "NO_MATCH a (undefined xs ys) ==> cvc_list_left (\<or>) xs (cvc_list_right (\<or>) False ys) =
+  shows "NO_MATCH cvc_a (undefined xs ys) \<Longrightarrow> cvc_list_left (\<or>) xs (cvc_list_right (\<or>) False ys) =
    cvc_list_both (\<or>) False xs ys"
   apply (cases ys)
   apply (cases xs)
@@ -92,11 +102,12 @@ lemma [rewrite_bool_or_false]:
     by (simp add: cvc_list_left_transfer cvc_list_right_transfer_op cvc_list_both_transfer_op)
   done
 
+
 named_theorems rewrite_bool_or_flatten \<open>automatically_generated\<close>
 
 lemma [rewrite_bool_or_flatten]:
   fixes xs::"bool cvc_ListVar" and b::"bool" and ys::"bool cvc_ListVar" and zs::"bool cvc_ListVar"
-  shows "NO_MATCH a (undefined xs b ys zs) ==> cvc_list_left (\<or>) xs
+  shows "NO_MATCH cvc_a (undefined xs b ys zs) \<Longrightarrow> cvc_list_left (\<or>) xs
     (cvc_list_right (\<or>) (cvc_list_right (\<or>) b ys) zs) =
    cvc_list_left (\<or>) xs (b \<or> cvc_list_both (\<or>) False ys zs)"
   apply (cases zs)
@@ -104,14 +115,21 @@ lemma [rewrite_bool_or_flatten]:
   apply (cases xs)
   subgoal for zss yss xss 
     apply (simp add: cvc_list_left_transfer cvc_list_right_transfer_op cvc_list_both_transfer_op)
-    by (metis foldr_or_neutral)
+    apply (induction zss)
+    apply simp_all
+    apply (induction yss)
+    apply simp_all
+    apply (induction xss)
+    apply simp_all
+    by (simp_all add: bool_or_flatten_lemma)
   done
+
 
 named_theorems rewrite_bool_or_dup \<open>automatically_generated\<close>
 
 lemma [rewrite_bool_or_dup]:
   fixes xs::"bool cvc_ListVar" and b::"bool" and ys::"bool cvc_ListVar" and zs::"bool cvc_ListVar"
-  shows "NO_MATCH a (undefined xs b ys zs) ==> cvc_list_left (\<or>) xs
+  shows "NO_MATCH cvc_a (undefined xs b ys zs) \<Longrightarrow> cvc_list_left (\<or>) xs
     (b \<or> cvc_list_left (\<or>) ys (cvc_list_right (\<or>) b zs)) =
    cvc_list_left (\<or>) xs (b \<or> cvc_list_both (\<or>) False ys zs)"
   apply (cases zs)
@@ -119,37 +137,46 @@ lemma [rewrite_bool_or_dup]:
   apply (cases xs)
   subgoal for zss yss xss 
     apply (simp add: cvc_list_left_transfer cvc_list_right_transfer_op cvc_list_both_transfer_op)
-    by (simp add: bool_or_dup_lemma)
+    apply (induction zss)
+    apply simp_all
+    apply (induction yss)
+    apply simp_all
+    apply (induction xss)
+    apply simp_all
+    by (simp_all add: bool_or_dup_lemma)
   done
+
 
 named_theorems rewrite_bool_and_true \<open>automatically_generated\<close>
 
 lemma [rewrite_bool_and_true]:
   fixes xs::"bool cvc_ListVar" and ys::"bool cvc_ListVar"
-  shows "NO_MATCH a (undefined xs ys) ==> cvc_list_left (\<and>) xs (cvc_list_right (\<and>) True ys) =
-         cvc_list_both (\<and>) True xs ys"
+  shows "NO_MATCH cvc_a (undefined xs ys) \<Longrightarrow> cvc_list_left (\<and>) xs (cvc_list_right (\<and>) True ys) =
+   cvc_list_both (\<and>) True xs ys"
   apply (cases ys)
   apply (cases xs)
   subgoal for yss xss 
     by (simp add: cvc_list_left_transfer cvc_list_right_transfer_op cvc_list_both_transfer_op)
   done
+
 
 named_theorems rewrite_bool_and_false \<open>automatically_generated\<close>
 
 lemma [rewrite_bool_and_false]:
   fixes xs::"bool cvc_ListVar" and ys::"bool cvc_ListVar"
-  shows "NO_MATCH a (undefined xs ys) ==> cvc_list_left (\<and>) xs (cvc_list_right (\<and>) False ys) = False"
+  shows "NO_MATCH cvc_a (undefined xs ys) \<Longrightarrow> cvc_list_left (\<and>) xs (cvc_list_right (\<and>) False ys) = False"
   apply (cases ys)
   apply (cases xs)
   subgoal for yss xss 
     by (simp add: cvc_list_left_transfer cvc_list_right_transfer_op cvc_list_both_transfer_op)
   done
 
+
 named_theorems rewrite_bool_and_flatten \<open>automatically_generated\<close>
 
 lemma [rewrite_bool_and_flatten]:
   fixes xs::"bool cvc_ListVar" and b::"bool" and ys::"bool cvc_ListVar" and zs::"bool cvc_ListVar"
-  shows "NO_MATCH a (undefined xs b ys zs) ==> cvc_list_left (\<and>) xs
+  shows "NO_MATCH cvc_a (undefined xs b ys zs) \<Longrightarrow> cvc_list_left (\<and>) xs
     (cvc_list_right (\<and>) (cvc_list_right (\<and>) b ys) zs) =
    cvc_list_left (\<and>) xs (b \<and> cvc_list_both (\<and>) True ys zs)"
   apply (cases zs)
@@ -157,14 +184,21 @@ lemma [rewrite_bool_and_flatten]:
   apply (cases xs)
   subgoal for zss yss xss 
     apply (simp add: cvc_list_left_transfer cvc_list_right_transfer_op cvc_list_both_transfer_op)
-    by (metis foldr_and_neutral)
+    apply (induction zss)
+    apply simp_all
+    apply (induction yss)
+    apply simp_all
+    apply (induction xss)
+    apply simp_all
+    by (simp_all add: bool_and_flatten_lemma)
   done
+
 
 named_theorems rewrite_bool_and_dup \<open>automatically_generated\<close>
 
 lemma [rewrite_bool_and_dup]:
   fixes xs::"bool cvc_ListVar" and b::"bool" and ys::"bool cvc_ListVar" and zs::"bool cvc_ListVar"
-  shows "NO_MATCH a (undefined xs b ys zs) ==> cvc_list_left (\<and>) xs
+  shows "NO_MATCH cvc_a (undefined xs b ys zs) \<Longrightarrow> cvc_list_left (\<and>) xs
     (b \<and> cvc_list_left (\<and>) ys (cvc_list_right (\<and>) b zs)) =
    cvc_list_left (\<and>) xs (b \<and> cvc_list_both (\<and>) True ys zs)"
   apply (cases zs)
@@ -172,14 +206,21 @@ lemma [rewrite_bool_and_dup]:
   apply (cases xs)
   subgoal for zss yss xss 
     apply (simp add: cvc_list_left_transfer cvc_list_right_transfer_op cvc_list_both_transfer_op)
-    by (simp add: bool_and_dup_lemma)
+    apply (induction zss)
+    apply simp_all
+    apply (induction yss)
+    apply simp_all
+    apply (induction xss)
+    apply simp_all
+    by (simp_all add: bool_and_dup_lemma)
   done
+
 
 named_theorems rewrite_bool_and_conf \<open>automatically_generated\<close>
 
 lemma [rewrite_bool_and_conf]:
   fixes xs::"bool cvc_ListVar" and w::"bool" and ys::"bool cvc_ListVar" and zs::"bool cvc_ListVar"
-  shows "NO_MATCH a (undefined xs w ys zs) ==> cvc_list_left (\<and>) xs
+  shows "NO_MATCH cvc_a (undefined xs w ys zs) \<Longrightarrow> cvc_list_left (\<and>) xs
     (w \<and>
      cvc_list_left (\<and>) ys (cvc_list_right (\<and>) (\<not> w) zs)) =
    False"
@@ -188,14 +229,21 @@ lemma [rewrite_bool_and_conf]:
   apply (cases xs)
   subgoal for zss yss xss 
     apply (simp add: cvc_list_left_transfer cvc_list_right_transfer_op cvc_list_both_transfer_op)
-    by (simp add: bool_and_conf_lemma)
+    apply (induction zss)
+    apply simp_all
+    apply (induction yss)
+    apply simp_all
+    apply (induction xss)
+    apply simp_all
+    by (simp_all add: bool_and_conf_lemma)
   done
+
 
 named_theorems rewrite_bool_or_taut \<open>automatically_generated\<close>
 
 lemma [rewrite_bool_or_taut]:
   fixes xs::"bool cvc_ListVar" and w::"bool" and ys::"bool cvc_ListVar" and zs::"bool cvc_ListVar"
-  shows "NO_MATCH a (undefined xs w ys zs) ==> cvc_list_left (\<or>) xs
+  shows "NO_MATCH cvc_a (undefined xs w ys zs) \<Longrightarrow> cvc_list_left (\<or>) xs
     (w \<or>
      cvc_list_left (\<or>) ys (cvc_list_right (\<or>) (\<not> w) zs)) =
    True"
@@ -204,98 +252,141 @@ lemma [rewrite_bool_or_taut]:
   apply (cases xs)
   subgoal for zss yss xss 
     apply (simp add: cvc_list_left_transfer cvc_list_right_transfer_op cvc_list_both_transfer_op)
-    by (simp add: bool_or_taut_lemma)
+    apply (induction zss)
+    apply simp_all
+    apply (induction yss)
+    apply simp_all
+    apply (induction xss)
+    apply simp_all
+    by (simp_all add: bool_or_taut_lemma)
   done
+
 
 named_theorems rewrite_bool_xor_refl \<open>automatically_generated\<close>
 
 lemma [rewrite_bool_xor_refl]:
   fixes x::"bool"
-  shows "NO_MATCH a (undefined x) ==> x [+] x = False"
-  using xor_def by auto
+  shows "NO_MATCH cvc_a (undefined x) \<Longrightarrow> (x \<noteq> x) = False"
+  by auto
+
 
 named_theorems rewrite_bool_xor_nrefl \<open>automatically_generated\<close>
 
 lemma [rewrite_bool_xor_nrefl]:
   fixes x::"bool"
-  shows "NO_MATCH a (undefined x) ==> x [+] (\<not> x) = True"
-  using xor_def by auto
+  shows "NO_MATCH cvc_a (undefined x) \<Longrightarrow> (x \<noteq> (\<not> x)) = True"
+  by auto
+
 
 named_theorems rewrite_bool_xor_false \<open>automatically_generated\<close>
 
 lemma [rewrite_bool_xor_false]:
   fixes x::"bool"
-  shows "NO_MATCH a (undefined x) ==> x [+] False = x"
-  using xor_def by auto
+  shows "NO_MATCH cvc_a (undefined x) \<Longrightarrow> (x \<noteq> False) = x"
+  by auto
+
 
 named_theorems rewrite_bool_xor_true \<open>automatically_generated\<close>
 
 lemma [rewrite_bool_xor_true]:
   fixes x::"bool"
-  shows "NO_MATCH a (undefined x) ==> x [+] True = (\<not> x)"
-  using xor_def by auto
+  shows "NO_MATCH cvc_a (undefined x) \<Longrightarrow> (x \<noteq> True) = (\<not> x)"
+  by auto
+
 
 named_theorems rewrite_bool_xor_comm \<open>automatically_generated\<close>
 
 lemma [rewrite_bool_xor_comm]:
   fixes x::"bool" and y::"bool"
-  shows "NO_MATCH a (undefined x) ==> x [+] y = y [+] x"
-  using xor_def by auto
+  shows "NO_MATCH cvc_a (undefined x y) \<Longrightarrow> (x \<noteq> y) = (y \<noteq> x)"
+  by auto
+
 
 named_theorems rewrite_bool_xor_elim \<open>automatically_generated\<close>
 
 lemma [rewrite_bool_xor_elim]:
   fixes x::"bool" and y::"bool"
-  shows "NO_MATCH a (undefined x) ==> x [+] y = (x \<noteq> y)"
-  using xor_def by auto
+  shows "NO_MATCH cvc_a (undefined x y) \<Longrightarrow> (x \<noteq> y) = (x \<noteq> y)"
+  by auto
+
 
 named_theorems rewrite_ite_neg_branch \<open>automatically_generated\<close>
 
 lemma [rewrite_ite_neg_branch]:
   fixes c::"bool" and x::"bool" and y::"bool"
-  shows "NO_MATCH a (undefined c x y) ==> (\<not> y) = x \<longrightarrow> (if c then x else y) = (c = x)"
+  shows "NO_MATCH cvc_a (undefined c x y) \<Longrightarrow> (\<not> y) = x \<longrightarrow> (if c then x else y) = (c = x)"
   by auto
+
 
 named_theorems rewrite_ite_then_true \<open>automatically_generated\<close>
 
 lemma [rewrite_ite_then_true]:
   fixes c::"bool" and x::"bool"
-  shows "NO_MATCH a (undefined c x) ==> (if c then True else x) = (c \<or> x)"
+  shows "NO_MATCH cvc_a (undefined c x) \<Longrightarrow> (if c then True else x) = (c \<or> x)"
   by auto
+
 
 named_theorems rewrite_ite_else_false \<open>automatically_generated\<close>
 
 lemma [rewrite_ite_else_false]:
   fixes c::"bool" and x::"bool"
-  shows "NO_MATCH a (undefined c x) ==> (if c then x else False) = (c \<and> x)"
+  shows "NO_MATCH cvc_a (undefined c x) \<Longrightarrow> (if c then x else False) = (c \<and> x)"
   by auto
+
 
 named_theorems rewrite_ite_then_false \<open>automatically_generated\<close>
 
 lemma [rewrite_ite_then_false]:
   fixes c::"bool" and x::"bool"
-  shows "NO_MATCH a (undefined c x) ==> (if c then False else x) = (\<not> c \<and> x)"
+  shows "NO_MATCH cvc_a (undefined c x) \<Longrightarrow> (if c then False else x) = (\<not> c \<and> x)"
   by auto
+
 
 named_theorems rewrite_ite_else_true \<open>automatically_generated\<close>
 
 lemma [rewrite_ite_else_true]:
   fixes c::"bool" and x::"bool"
-  shows "NO_MATCH a (undefined c x) ==> (if c then x else True) = (\<not> c \<or> x)"
+  shows "NO_MATCH cvc_a (undefined c x) \<Longrightarrow> (if c then x else True) = (\<not> c \<or> x)"
   by auto
+
 
 named_theorems rewrite_ite_then_lookahead_self \<open>automatically_generated\<close>
 
 lemma [rewrite_ite_then_lookahead_self]:
   fixes c::"bool" and x::"bool"
-  shows "NO_MATCH a (undefined c x) ==> (if c then c else x) = (if c then True else x)"
+  shows "NO_MATCH cvc_a (undefined c x) \<Longrightarrow> (if c then c else x) = (if c then True else x)"
   by auto
+
 
 named_theorems rewrite_ite_else_lookahead_self \<open>automatically_generated\<close>
 
 lemma [rewrite_ite_else_lookahead_self]:
   fixes c::"bool" and x::"bool"
-  shows "NO_MATCH a (undefined c x) ==> (if c then x else c) = (if c then x else False)"
+  shows "NO_MATCH cvc_a (undefined c x) \<Longrightarrow> (if c then x else c) = (if c then x else False)"
+  by auto
+
+
+named_theorems rewrite_bool_commutative_and \<open>automatically_generated\<close>
+
+lemma [rewrite_bool_commutative_and]:
+  fixes x::"bool" and y::"bool"
+  shows "NO_MATCH cvc_a (undefined x y) \<Longrightarrow> (x \<and> y) = (y \<and> x)"
+  by auto
+
+
+named_theorems rewrite_bool_commutative_or \<open>automatically_generated\<close>
+
+lemma [rewrite_bool_commutative_or]:
+  fixes x::"bool" and y::"bool"
+  shows "NO_MATCH cvc_a (undefined x y) \<Longrightarrow> (x \<or> y) = (y \<or> x)"
+  by auto
+
+
+named_theorems rewrite_bool_commutative_xor \<open>automatically_generated\<close>
+
+lemma [rewrite_bool_commutative_xor]:
+  fixes x::"bool" and y::"bool"
+  shows "NO_MATCH cvc_a (undefined x y) \<Longrightarrow> (x \<noteq> y) = (y \<noteq> x)"
   by auto
 
 end
