src/HOL/CVC/cvc5_dsl_rewrites/Boolean_Rewrites_Lemmas.thy
@@ -2,81 +2,46 @@ theory Boolean_Rewrites_Lemmas
   imports Dsl_Nary_Ops
 begin
 
-lemma foldr_or_neutral [simp]: "foldr (\<or>) xs True = True"
-  apply (induction xs)
-  by auto
-
-lemma foldr_and_neutral [simp]: "foldr (\<and>) xs False = False"
-  apply (induction xs)
-  by auto
-
-lemma bool_or_taut_lemma: 
-  "foldr (\<or>) xss (w \<or> foldr (\<or>) yss (w \<longrightarrow> foldr (\<or>) zss False))"
-    apply (induction zss)
-     apply (induction yss)
-     apply (induction xss)
-     apply simp_all
-  apply (metis (mono_tags, lifting) foldr_or_neutral)
-  by metis
-
+lemma bool_or_taut_lemma:
+ "w \<or> a \<or> foldr (\<or>) yss (\<not> w)"
+ "a \<or> foldr (\<or>) xss (w \<or> aa \<or> foldr (\<or>) yss (\<not> w))"
+ "foldr (\<or>) xss (w \<or> foldr (\<or>) yss (w \<longrightarrow> a \<or> foldr (\<or>) zss False))"
+    apply force
+   apply (metis (mono_tags, opaque_lifting) foldr_or_neutral)
+  by (metis foldr_or_neutral)
 
 lemma bool_and_conf_lemma:
-  "\<not> foldr (\<and>) xss (w \<and> foldr (\<and>) yss (\<not> w \<and> foldr (\<and>) zss True))"
-  apply (induction zss)
-   apply (induction yss)
-    apply (induction xss)
-     apply simp_all
-   apply (metis (mono_tags, lifting) foldr_and_neutral)
-  by (metis (mono_tags, lifting))
-
+ "\<not> foldr (\<and>) xss (w \<and> aa \<and> foldr (\<and>) yss (\<not> w))"
+ "\<not> foldr (\<and>) xss (w \<and> foldr (\<and>) yss (\<not> w \<and> a \<and> foldr (\<and>) zss True))"
+  apply (metis (mono_tags, opaque_lifting) foldr_and_neutral)
+  by (metis(full_types) foldr_and_neutral)
 
 lemma bool_and_dup_lemma:
-  "foldr (\<and>) xss (b \<and> foldr (\<and>) yss (b \<and> foldr (\<and>) zss True))
- = foldr (\<and>) xss (b \<and> foldr (\<and>) yss (foldr (\<and>) zss True))"
-  apply (induction zss)
-   apply (induction yss)
-    apply (induction xss)
-     apply simp_all
-  apply metis
-  by metis
+  "(b \<and> a \<and> foldr (\<and>) yss b) = (b \<and> a \<and> foldr (\<and>) yss True)"
+  "(a \<and> foldr (\<and>) xss (b \<and> aa \<and> foldr (\<and>) yss b)) = (a \<and> foldr (\<and>) xss (b \<and> aa \<and> foldr (\<and>) yss True))"
+  "foldr (\<and>) xss (b \<and> foldr (\<and>) yss (b \<and> a \<and> foldr (\<and>) zss True)) = foldr (\<and>) xss (b \<and> foldr (\<and>) yss (a \<and> foldr (\<and>) zss True))"
+   apply auto[1]
+   apply (metis(full_types))
+  by (metis(full_types))
 
 lemma bool_and_flatten_lemma:
-  "foldr (\<and>) xss (b \<and> foldr (\<and>) yss True \<and> foldr (\<and>) zss True)
-  = foldr (\<and>) xss (foldr (\<and>) zss (b \<and> foldr (\<and>) yss True))"
-    apply (induction zss)
-     apply simp_all
-     apply (induction yss)
-      apply simp_all
-     apply (induction xss)
-      apply simp_all
-    apply (metis foldr_and_neutral)
-     apply (metis foldr_and_neutral)
-    by (metis foldr_and_neutral)
+  " (b \<and> a \<and> foldr (\<and>) yss True \<and> aa \<and> foldr (\<and>) zss True) = (b \<and> a \<and> foldr (\<and>) yss (aa \<and> foldr (\<and>) zss True))"
+  by (metis(full_types) foldr_and_neutral)
 
 lemma bool_or_dup_lemma:
-  "foldr (\<or>) xss (b \<or> foldr (\<or>) yss (b \<or> foldr (\<or>) zss False))
- = foldr (\<or>) xss (b \<or> foldr (\<or>) yss (foldr (\<or>) zss False))"
-  apply (induction zss)
-   apply simp_all
-     apply (induction yss)
-      apply simp_all
-     apply (induction xss)
-      apply simp_all
-    apply blast
-  apply blast
-  by (metis foldr_or_neutral)
+  "(b \<or> a \<or> foldr (\<or>) yss b) = (b \<or> a \<or> foldr (\<or>) yss False)"
+  "(a \<or> foldr (\<or>) xss (b \<or> aa \<or> foldr (\<or>) yss b)) = (a \<or> foldr (\<or>) xss (b \<or> aa \<or> foldr (\<or>) yss False))"
+  "foldr (\<or>) xss (b \<or> foldr (\<or>) yss (b \<or> a \<or> foldr (\<or>) zss False)) = foldr (\<or>) xss (b \<or> foldr (\<or>) yss (a \<or> foldr (\<or>) zss False))"
+    apply auto[1]
+   apply (metis(full_types))
+  by (metis(full_types))
 
 lemma bool_or_flatten_lemma:
-  "foldr (\<or>) xss (b \<or> foldr (\<or>) yss False \<or> foldr (\<or>) zss False)
- = foldr (\<or>) xss (foldr (\<or>) zss (b \<or> foldr (\<or>) yss False))"
-  apply (induction zss)
-   apply simp_all
-     apply (induction yss)
-      apply simp_all
-     apply (induction xss)
-      apply simp_all
-    apply blast
-  apply blast
-  by (metis foldr_or_neutral)
+ "(b \<or> a \<or> foldr (\<or>) yss False \<or> aa \<or> foldr (\<or>) zss False) = (b \<or> a \<or> foldr (\<or>) yss (aa \<or> foldr (\<or>) zss False))"
+ "(a \<or> foldr (\<or>) xss (b \<or> aa \<or> foldr (\<or>) yss False \<or> aaa \<or> foldr (\<or>) zss False)) =
+  (a \<or> foldr (\<or>) xss (b \<or> aa \<or> foldr (\<or>) yss (aaa \<or> foldr (\<or>) zss False)))"
+   apply (metis(full_types) foldr_or_neutral)
+  by (metis(full_types) foldr_or_neutral)
+ 
 
 end
