src/HOL/CVC/cvc5_dsl_rewrites/String_Rewrites.thy
@@ -1,25 +1,16 @@
 theory String_Rewrites
-  imports Dsl_Nary_Ops String_Rewrites_Lemmas
+  imports "HOL-CVC.Dsl_Nary_Ops"  "String_Rewrites_Lemmas"
 begin
 
-(* This is a theory automatically created from a rare file! All that remains to do is to prove
-any lemma whose provided proof fails and to to import this file in SMT.thy. 
-If your rare statements use nary operators over lists that would be binarised by Isabelle 
-you have to add it in Dsl_Nary_Ops.thy. Currently already supported are the operators:
-and,
-or,
-plus,
-times,
-append,
-re_concat,
-str_concat,
-*)
+(* Thank you for using IsaRARE. This is a theory automatically created from a RARE file!
+All that remains to do is to prove any lemma whose provided proof fails.
+If you want to use the lemmas for proof reconstruction you'll also need to import this file in Rare_Interface.thy*)
 
 named_theorems rewrite_str_eq_ctn_false \<open>automatically_generated\<close>
 
 lemma [rewrite_str_eq_ctn_false]:
   fixes x1::"char list cvc_ListVar" and x::"char list" and x2::"char list cvc_ListVar" and y::"char list"
-  shows "smtlib_str_contains y x = False \<longrightarrow>
+  shows "NO_MATCH cvc_a (undefined x1 x x2 y) \<Longrightarrow> smtlib_str_contains y x = False \<longrightarrow>
    (cvc_list_right smtlib_str_concat (cvc_list_left smtlib_str_concat x1 x)
      x2 =
     y) =
@@ -28,14 +19,21 @@ lemma [rewrite_str_eq_ctn_false]:
   apply (cases x1)
   subgoal for x2s x1s 
     apply (simp add: cvc_list_left_transfer cvc_list_right_transfer_op cvc_list_both_transfer_op)
-    by (simp add: str_eq_ctn_false_lemma)
+    apply (induction x2s arbitrary: x2)
+    apply simp_all
+    apply (induction x1s arbitrary: x1)
+    apply simp_all
+    apply (simp_all add: cvc_string_rewrite_defs)
+      apply (simp_all add: cvc_rewrites_fold)
+    by (simp_all add: str_eq_ctn_false_lemma)
   done
+
 
 named_theorems rewrite_str_concat_flatten \<open>automatically_generated\<close>
 
 lemma [rewrite_str_concat_flatten]:
   fixes xs::"char list cvc_ListVar" and s::"char list" and ys::"char list cvc_ListVar" and zs::"char list cvc_ListVar"
-  shows "cvc_list_right smtlib_str_concat
+  shows "NO_MATCH cvc_a (undefined xs s ys zs) \<Longrightarrow> cvc_list_right smtlib_str_concat
     (cvc_list_left smtlib_str_concat xs
       (cvc_list_right smtlib_str_concat s ys))
     zs =
@@ -48,14 +46,22 @@ lemma [rewrite_str_concat_flatten]:
   apply (cases xs)
   subgoal for zss yss xss 
     apply (simp add: cvc_list_left_transfer cvc_list_right_transfer_op cvc_list_both_transfer_op)
-    by (simp add: str_concat_flatten_lemma)
+    apply (induction zss arbitrary: zs)
+    apply simp_all
+    apply (induction yss arbitrary: ys)
+    apply simp_all
+    apply (induction xss arbitrary: xs)
+    apply simp_all
+    apply (simp_all add: cvc_string_rewrite_defs)
+    by (simp_all add: cvc_rewrites_fold)
   done
+
 
 named_theorems rewrite_str_concat_flatten_eq \<open>automatically_generated\<close>
 
 lemma [rewrite_str_concat_flatten_eq]:
   fixes x::"char list" and x1::"char list cvc_ListVar" and x2::"char list cvc_ListVar" and y::"char list"
-  shows "(cvc_list_right smtlib_str_concat (cvc_list_right smtlib_str_concat x x1)
+  shows "NO_MATCH cvc_a (undefined x x1 x2 y) \<Longrightarrow> (cvc_list_right smtlib_str_concat (cvc_list_right smtlib_str_concat x x1)
      x2 =
     y) =
    (y =
@@ -65,14 +71,21 @@ lemma [rewrite_str_concat_flatten_eq]:
   apply (cases x1)
   subgoal for x2s x1s 
     apply (simp add: cvc_list_left_transfer cvc_list_right_transfer_op cvc_list_both_transfer_op)
-    by (simp add: str_concat_flatten_eq_lemma)
+    apply (induction x2s arbitrary: x2)
+    apply simp_all
+    apply (induction x1s arbitrary: x1)
+    apply simp_all
+    apply (simp_all add: cvc_string_rewrite_defs)
+    apply (simp_all add: cvc_rewrites_fold)
+    by (simp_all add: str_concat_flatten_eq_lemma)
   done
+
 
 named_theorems rewrite_str_concat_flatten_eq_rev \<open>automatically_generated\<close>
 
 lemma [rewrite_str_concat_flatten_eq_rev]:
   fixes x::"char list" and x1::"char list cvc_ListVar" and x2::"char list cvc_ListVar" and y::"char list"
-  shows "(cvc_list_left smtlib_str_concat x2
+  shows "NO_MATCH cvc_a (undefined x x1 x2 y) \<Longrightarrow> (cvc_list_left smtlib_str_concat x2
      (cvc_list_left smtlib_str_concat x1 x) =
     y) =
    (y = smtlib_str_concat (cvc_list_both smtlib_str_concat [] x2 x1) x)"
@@ -80,58 +93,60 @@ lemma [rewrite_str_concat_flatten_eq_rev]:
   apply (cases x1)
   subgoal for x2s x1s 
     apply (simp add: cvc_list_left_transfer cvc_list_right_transfer_op cvc_list_both_transfer_op)
-    by (simp add: str_concat_flatten_eq_rev_lemma)
-  done                              
+    apply (induction x2s arbitrary: x2)
+    apply simp_all
+    apply (induction x1s arbitrary: x1)
+    apply simp_all
+    apply (simp_all add: cvc_string_rewrite_defs)
+    apply (simp_all add: cvc_rewrites_fold)
+    by auto
+  done
+
 
 named_theorems rewrite_str_substr_empty_str \<open>automatically_generated\<close>
 
 lemma [rewrite_str_substr_empty_str]:
   fixes n::"int" and m::"int"
-  shows "smtlib_str_substr (''''::char list) n m = ''''"
-  unfolding smtlib_str_substr_def
-  by simp
+  shows "NO_MATCH cvc_a (undefined n m) \<Longrightarrow> smtlib_str_substr (''''::char list) n m = ''''"
+    by (simp add: cvc_string_rewrite_defs)
 
 named_theorems rewrite_str_substr_empty_range \<open>automatically_generated\<close>
 
 lemma [rewrite_str_substr_empty_range]:
   fixes x::"char list" and n::"int" and m::"int"
-  shows "m \<le> (0::int) \<longrightarrow>
+  shows "NO_MATCH cvc_a (undefined x n m) \<Longrightarrow> m \<le> (0::int) \<longrightarrow>
    smtlib_str_substr x n m = (''''::char list)"
-  unfolding smtlib_str_substr_def
-  by simp
+    by (simp add: cvc_string_rewrite_defs)
 
 named_theorems rewrite_str_substr_empty_start \<open>automatically_generated\<close>
 
 lemma [rewrite_str_substr_empty_start]:
   fixes x::"char list" and n::"int" and m::"int"
-  shows "smtlib_str_len x \<le> n \<longrightarrow>
+  shows "NO_MATCH cvc_a (undefined x n m) \<Longrightarrow> smtlib_str_len x \<le> n \<longrightarrow>
    smtlib_str_substr x n m = (''''::char list)"
-  unfolding smtlib_str_substr_def smtlib_str_len_def
-  by simp
+    by (simp add: cvc_string_rewrite_defs)
 
 named_theorems rewrite_str_substr_empty_start_neg \<open>automatically_generated\<close>
 
 lemma [rewrite_str_substr_empty_start_neg]:
   fixes x::"char list" and n::"int" and m::"int"
-  shows "n < (0::int) \<longrightarrow>
+  shows "NO_MATCH cvc_a (undefined x n m) \<Longrightarrow> n < (0::int) \<longrightarrow>
    smtlib_str_substr x n m = (''''::char list)"
-  unfolding smtlib_str_substr_def smtlib_str_len_def
-  by simp
+    by (simp add: cvc_string_rewrite_defs)
 
 named_theorems rewrite_str_substr_eq_empty \<open>automatically_generated\<close>
 
 lemma [rewrite_str_substr_eq_empty]:
   fixes s::"char list" and n::"int" and m::"int"
-  shows "n = (0::int) \<and> n < m \<longrightarrow>
+  shows "NO_MATCH cvc_a (undefined s n m) \<Longrightarrow> n = (0::int) \<and> n < m \<longrightarrow>
    (smtlib_str_substr s n m = (''''::char list)) = (s = '''')"
-  unfolding smtlib_str_substr_def smtlib_str_len_def
-  by simp
+    by (simp add: cvc_string_rewrite_defs)
 
 named_theorems rewrite_str_len_replace_inv \<open>automatically_generated\<close>
 
 lemma [rewrite_str_len_replace_inv]:
   fixes t::"char list" and s::"char list" and r::"char list"
-  shows "smtlib_str_len s = smtlib_str_len r \<longrightarrow>
+  shows "NO_MATCH cvc_a (undefined t s r) \<Longrightarrow> smtlib_str_len s = smtlib_str_len r \<longrightarrow>
    smtlib_str_len (smtlib_str_replace t s r) = smtlib_str_len t"
   using smtlib_str_len_def smtlib_str_replace_def smtlib_str_replace_length by presburger
 
@@ -139,75 +154,78 @@ named_theorems rewrite_str_len_update_inv \<open>automatically_generated\<close>
 
 lemma [rewrite_str_len_update_inv]:
   fixes t::"char list" and n::"int" and r::"char list"
-  shows "smtlib_str_len (smtlib_str_update t n r) = smtlib_str_len t"
-  unfolding smtlib_str_update_def smtlib_str_len_def Let_def
-  by force
+  shows "NO_MATCH cvc_a (undefined t n r) \<Longrightarrow> smtlib_str_len (smtlib_str_update t n r) = smtlib_str_len t"
+  apply (simp add: cvc_string_rewrite_defs)
+  by auto
 
 named_theorems rewrite_str_len_substr_in_range \<open>automatically_generated\<close>
 
 lemma [rewrite_str_len_substr_in_range]:
   fixes s::"char list" and n::"int" and m::"int"
-  shows "(0::int) \<le> n \<and>
+  shows "NO_MATCH cvc_a (undefined s n m) \<Longrightarrow> (0::int) \<le> n \<and>
    (0::int) \<le> m \<and> n + m \<le> smtlib_str_len s \<longrightarrow>
    smtlib_str_len (smtlib_str_substr s n m) = m"
-  using smtlib_str_len_def smtlib_str_substr_length by force
+  apply (simp add: cvc_string_rewrite_defs)
+  by auto
 
 named_theorems rewrite_str_len_substr_ub1 \<open>automatically_generated\<close>
 
 lemma [rewrite_str_len_substr_ub1]:
   fixes s::"char list" and n::"int" and m::"int" and k::"int"
-  shows "m \<le> k \<longrightarrow> k \<ge> 0 \<longrightarrow>
+  shows "NO_MATCH cvc_a (undefined s n m k) \<Longrightarrow> (0::int) \<le> k \<and> m \<le> k \<longrightarrow>
    (smtlib_str_len (smtlib_str_substr s n m) \<le> k) = True"
-  by (simp add: min_def nat_le_iff)
+  apply (simp add: cvc_string_rewrite_defs)
+  by auto
 
 named_theorems rewrite_str_len_substr_ub2 \<open>automatically_generated\<close>
 
 lemma [rewrite_str_len_substr_ub2]:
   fixes s::"char list" and n::"int" and m::"int" and k::"int"
-  shows "smtlib_str_len s - n \<le> k \<longrightarrow> k \<ge> 0 \<longrightarrow>
+  shows "NO_MATCH cvc_a (undefined s n m k) \<Longrightarrow> (0::int) \<le> k \<and> smtlib_str_len s - n \<le> k \<longrightarrow>
    (smtlib_str_len (smtlib_str_substr s n m) \<le> k) = True"
-  using smtlib_str_len_def smtlib_str_substr_length by auto
+  apply (simp add: cvc_string_rewrite_defs)
+  by auto
 
 named_theorems rewrite_re_in_empty \<open>automatically_generated\<close>
 
 lemma [rewrite_re_in_empty]:
   fixes t::"char list"
-  shows "smtlib_str_in_re t smtlib_re_none = False"
-  by (simp add: smtlib_re_none_def smtlib_str_in_re_def)
+  shows "NO_MATCH cvc_a (undefined t) \<Longrightarrow> smtlib_str_in_re t smtlib_re_none = False"
+    by (simp add: cvc_string_rewrite_defs)
 
 named_theorems rewrite_re_in_sigma \<open>automatically_generated\<close>
 
 lemma [rewrite_re_in_sigma]:
   fixes t::"char list"
-  shows "smtlib_str_in_re t smtlib_re_allchar = (smtlib_str_len t = (1::int))"
-  by (simp add: smtlib_re_allchar_def smtlib_str_in_re_def smtlib_str_len_def)
+  shows "NO_MATCH cvc_a (undefined t) \<Longrightarrow> smtlib_str_in_re t smtlib_re_allchar = (smtlib_str_len t = (1::int))"
+    by (simp add: cvc_string_rewrite_defs)
 
 named_theorems rewrite_re_in_sigma_star \<open>automatically_generated\<close>
 
 lemma [rewrite_re_in_sigma_star]:
   fixes t::"char list"
-  shows "smtlib_str_in_re t (smtlib_re_star smtlib_re_allchar) = True"
+  shows "NO_MATCH cvc_a (undefined t) \<Longrightarrow> smtlib_str_in_re t (smtlib_re_star smtlib_re_allchar) = True"
   by (simp add: smtlib_str_in_re_def)
 
 named_theorems rewrite_re_in_cstring \<open>automatically_generated\<close>
 
 lemma [rewrite_re_in_cstring]:
   fixes t::"char list" and s::"char list"
-  shows "smtlib_str_in_re t (smtlib_str_to_re s) = (t = s)"
-  by (simp add: smtlib_str_in_re_def smtlib_str_to_re_def)
+  shows "NO_MATCH cvc_a (undefined t s) \<Longrightarrow> smtlib_str_in_re t (smtlib_str_to_re s) = (t = s)"
+    by (simp add: cvc_string_rewrite_defs)
 
 named_theorems rewrite_re_in_comp \<open>automatically_generated\<close>
 
 lemma [rewrite_re_in_comp]:
   fixes t::"char list" and r::"char list set"
-  shows "smtlib_str_in_re t (smtlib_re_comp r) = (\<not> smtlib_str_in_re t r)"
-  by (simp add: smtlib_re_comp_def smtlib_str_in_re_def)
+  shows "NO_MATCH cvc_a (undefined t r) \<Longrightarrow> smtlib_str_in_re t (smtlib_re_comp r) = (\<not> smtlib_str_in_re t r)"
+    by (simp add: cvc_string_rewrite_defs)
 
 named_theorems rewrite_str_concat_clash \<open>automatically_generated\<close>
 
 lemma [rewrite_str_concat_clash]:
   fixes s1::"char list" and s2::"char list cvc_ListVar" and t1::"char list" and t2::"char list cvc_ListVar"
-  shows "s1 \<noteq> t1 \<and>
+  shows "NO_MATCH cvc_a (undefined s1 s2 t1 t2) \<Longrightarrow> s1 \<noteq> t1 \<and>
    smtlib_str_len s1 = smtlib_str_len t1 \<longrightarrow>
    (cvc_list_right smtlib_str_concat s1 s2 =
     cvc_list_right smtlib_str_concat t1 t2) =
@@ -216,14 +234,21 @@ lemma [rewrite_str_concat_clash]:
   apply (cases s2)
   subgoal for t2s s2s 
     apply (simp add: cvc_list_left_transfer cvc_list_right_transfer_op cvc_list_both_transfer_op)
-    by (simp add: concat_clash_lemma)
+    apply (induction t2s arbitrary: t2)
+    apply simp_all
+    apply (induction s2s arbitrary: s2)
+    apply simp_all
+    apply (simp_all add: cvc_string_rewrite_defs)
+    apply (simp_all add: cvc_rewrites_fold)
+    by auto
   done
+
 
 named_theorems rewrite_str_concat_clash_rev \<open>automatically_generated\<close>
 
 lemma [rewrite_str_concat_clash_rev]:
   fixes s1::"char list" and s2::"char list cvc_ListVar" and t1::"char list" and t2::"char list cvc_ListVar"
-  shows "s1 \<noteq> t1 \<and>
+  shows "NO_MATCH cvc_a (undefined s1 s2 t1 t2) \<Longrightarrow> s1 \<noteq> t1 \<and>
    smtlib_str_len s1 = smtlib_str_len t1 \<longrightarrow>
    (cvc_list_left smtlib_str_concat s2 s1 =
     cvc_list_left smtlib_str_concat t2 t1) =
@@ -232,40 +257,58 @@ lemma [rewrite_str_concat_clash_rev]:
   apply (cases s2)
   subgoal for t2s s2s 
     apply (simp add: cvc_list_left_transfer cvc_list_right_transfer_op cvc_list_both_transfer_op)
-    by (simp add: concat_clash_rev_lemma)
+    apply (induction t2s arbitrary: t2)
+    apply simp_all
+    apply (induction s2s arbitrary: s2)
+    apply simp_all
+    apply (simp_all add: cvc_string_rewrite_defs)
+     apply (simp_all add: cvc_rewrites_fold)
+     apply auto
+    by (metis append.assoc append_eq_append_conv)
   done
+
 
 named_theorems rewrite_str_concat_clash2 \<open>automatically_generated\<close>
 
 lemma [rewrite_str_concat_clash2]:
   fixes s1::"char list" and t1::"char list" and t2::"char list cvc_ListVar"
-  shows "s1 \<noteq> t1 \<and>
+  shows "NO_MATCH cvc_a (undefined s1 t1 t2) \<Longrightarrow> s1 \<noteq> t1 \<and>
    smtlib_str_len s1 = smtlib_str_len t1 \<longrightarrow>
    (s1 = cvc_list_right smtlib_str_concat t1 t2) = False"
   apply (cases t2)
   subgoal for t2s 
     apply (simp add: cvc_list_left_transfer cvc_list_right_transfer_op cvc_list_both_transfer_op)
-    by (simp add: concat_clash2_lemma)
+    apply (induction t2s arbitrary: t2)
+    apply simp_all
+    apply (simp_all add: cvc_string_rewrite_defs)
+    apply (simp_all add: cvc_rewrites_fold)
+    by auto
   done
+
 
 named_theorems rewrite_str_concat_clash2_rev \<open>automatically_generated\<close>
 
 lemma [rewrite_str_concat_clash2_rev]:
   fixes s1::"char list" and t1::"char list" and t2::"char list cvc_ListVar"
-  shows "s1 \<noteq> t1 \<and>
+  shows "NO_MATCH cvc_a (undefined s1 t1 t2) \<Longrightarrow> s1 \<noteq> t1 \<and>
    smtlib_str_len s1 = smtlib_str_len t1 \<longrightarrow>
    (s1 = cvc_list_left smtlib_str_concat t2 t1) = False"
   apply (cases t2)
   subgoal for t2s 
     apply (simp add: cvc_list_left_transfer cvc_list_right_transfer_op cvc_list_both_transfer_op)
-    by (simp add: concat_clash2_rev_lemma)
+    apply (induction t2s arbitrary: t2)
+    apply simp_all
+    apply (simp_all add: cvc_string_rewrite_defs)
+    apply (simp_all add: cvc_rewrites_fold)
+    by auto
   done
+
 
 named_theorems rewrite_str_concat_unify \<open>automatically_generated\<close>
 
 lemma [rewrite_str_concat_unify]:
   fixes s1::"char list" and s2::"char list" and s3::"char list cvc_ListVar" and t2::"char list" and t3::"char list cvc_ListVar"
-  shows "(cvc_list_right smtlib_str_concat (smtlib_str_concat s1 s2) s3 =
+  shows "NO_MATCH cvc_a (undefined s1 s2 s3 t2 t3) \<Longrightarrow> (cvc_list_right smtlib_str_concat (smtlib_str_concat s1 s2) s3 =
     cvc_list_right smtlib_str_concat (smtlib_str_concat s1 t2) t3) =
    (cvc_list_right smtlib_str_concat s2 s3 =
     cvc_list_right smtlib_str_concat t2 t3)"
@@ -273,14 +316,19 @@ lemma [rewrite_str_concat_unify]:
   apply (cases s3)
   subgoal for t3s s3s 
     apply (simp add: cvc_list_left_transfer cvc_list_right_transfer_op cvc_list_both_transfer_op)
-    by (simp add: concat_unify_lemma)
+    apply (induction t3s arbitrary: t3)
+    apply simp_all
+    apply (induction s3s arbitrary: s3)
+    apply simp_all
+    by (simp_all add: cvc_string_rewrite_defs)
   done
+
 
 named_theorems rewrite_str_concat_unify_rev \<open>automatically_generated\<close>
 
 lemma [rewrite_str_concat_unify_rev]:
   fixes s1::"char list" and s2::"char list" and s3::"char list cvc_ListVar" and t2::"char list" and t3::"char list cvc_ListVar"
-  shows "(smtlib_str_concat (cvc_list_right smtlib_str_concat s2 s3) s1 =
+  shows "NO_MATCH cvc_a (undefined s1 s2 s3 t2 t3) \<Longrightarrow> (smtlib_str_concat (cvc_list_right smtlib_str_concat s2 s3) s1 =
     smtlib_str_concat (cvc_list_right smtlib_str_concat t2 t3) s1) =
    (cvc_list_right smtlib_str_concat s2 s3 =
     cvc_list_right smtlib_str_concat t2 t3)"
@@ -288,14 +336,19 @@ lemma [rewrite_str_concat_unify_rev]:
   apply (cases s3)
   subgoal for t3s s3s 
     apply (simp add: cvc_list_left_transfer cvc_list_right_transfer_op cvc_list_both_transfer_op)
-    by (simp add: concat_unify_rev_lemma)
+    apply (induction t3s arbitrary: t3)
+    apply simp_all
+    apply (induction s3s arbitrary: s3)
+    apply simp_all
+    by (simp_all add: cvc_string_rewrite_defs)
   done
+
 
 named_theorems rewrite_str_concat_clash_char \<open>automatically_generated\<close>
 
 lemma [rewrite_str_concat_clash_char]:
   fixes s1::"char list" and s2::"char list cvc_ListVar" and s3::"char list cvc_ListVar" and t1::"char list" and t2::"char list cvc_ListVar" and t3::"char list cvc_ListVar"
-  shows "s1 \<noteq> t1 \<and>
+  shows "NO_MATCH cvc_a (undefined s1 s2 s3 t1 t2 t3) \<Longrightarrow> s1 \<noteq> t1 \<and>
    smtlib_str_len s1 = smtlib_str_len t1 \<longrightarrow>
    (cvc_list_right smtlib_str_concat
      (cvc_list_right smtlib_str_concat s1 s2) s3 =
@@ -308,14 +361,26 @@ lemma [rewrite_str_concat_clash_char]:
   apply (cases s2)
   subgoal for t3s t2s s3s s2s 
     apply (simp add: cvc_list_left_transfer cvc_list_right_transfer_op cvc_list_both_transfer_op)
-    by (simp add: concat_clash_char_lemma)
+    apply (induction t3s arbitrary: t3)
+    apply simp_all
+    apply (induction t2s arbitrary: t2)
+    apply simp_all
+    apply (induction s3s arbitrary: s3)
+    apply simp_all
+    apply (induction s2s arbitrary: s2)
+    apply simp_all
+    apply (simp_all add: cvc_string_rewrite_defs)
+     apply (simp_all add: cvc_rewrites_fold)
+     apply (simp add: append_eq_conv_conj)
+    by (simp add: append_eq_conv_conj)
   done
+
 
 named_theorems rewrite_str_concat_clash_char_rev \<open>automatically_generated\<close>
 
 lemma [rewrite_str_concat_clash_char_rev]:
   fixes s1::"char list" and s2::"char list cvc_ListVar" and s3::"char list cvc_ListVar" and t1::"char list" and t2::"char list cvc_ListVar" and t3::"char list cvc_ListVar"
-  shows "s1 \<noteq> t1 \<and>
+  shows "NO_MATCH cvc_a (undefined s1 s2 s3 t1 t2 t3) \<Longrightarrow> s1 \<noteq> t1 \<and>
    smtlib_str_len s1 = smtlib_str_len t1 \<longrightarrow>
    (cvc_list_left smtlib_str_concat s3
      (cvc_list_left smtlib_str_concat s2 s1) =
@@ -331,19 +396,20 @@ lemma [rewrite_str_concat_clash_char_rev]:
     by (simp add: concat_clash_char_rev_lemma)
   done
 
+
 named_theorems rewrite_str_prefixof_elim \<open>automatically_generated\<close>
 
 lemma [rewrite_str_prefixof_elim]:
   fixes s::"char list" and t::"char list"
-  shows "smtlib_str_prefixof s t =
+  shows "NO_MATCH cvc_a (undefined s t) \<Longrightarrow> smtlib_str_prefixof s t =
    (s = smtlib_str_substr t (0::int) (smtlib_str_len s))"
-  by (simp add: rewrite_str_prefixof_elim_lemma)
+   by (simp add: rewrite_str_prefixof_elim_lemma)
 
 named_theorems rewrite_str_suffixof_elim \<open>automatically_generated\<close>
 
 lemma [rewrite_str_suffixof_elim]:
   fixes s::"char list" and t::"char list"
-  shows "smtlib_str_suffixof s t =
+  shows "NO_MATCH cvc_a (undefined s t) \<Longrightarrow> smtlib_str_suffixof s t =
    (s =
     smtlib_str_substr t (smtlib_str_len t - smtlib_str_len s)
      (smtlib_str_len s))"
@@ -353,27 +419,27 @@ named_theorems rewrite_str_prefixof_one \<open>automatically_generated\<close>
 
 lemma [rewrite_str_prefixof_one]:
   fixes s::"char list" and t::"char list"
-  shows "smtlib_str_len t = (1::int) \<longrightarrow>
+  shows "NO_MATCH cvc_a (undefined s t) \<Longrightarrow> smtlib_str_len t = (1::int) \<longrightarrow>
    smtlib_str_prefixof s t = smtlib_str_contains t s"
-   by (simp add: smtlib_str_contains2_def smtlib_str_contains_equal smtlib_str_len_def smtlib_str_prefixof_def str_prefixof_one_lemma)
+  by (simp add: smtlib_str_contains2_def smtlib_str_contains_equal smtlib_str_len_def smtlib_str_prefixof_def str_prefixof_one_lemma)
 
 named_theorems rewrite_str_suffixof_one \<open>automatically_generated\<close>
 
 lemma [rewrite_str_suffixof_one]:
   fixes s::"char list" and t::"char list"
-  shows "smtlib_str_len t = (1::int) \<longrightarrow>
+  shows "NO_MATCH cvc_a (undefined s t) \<Longrightarrow> smtlib_str_len t = (1::int) \<longrightarrow>
    smtlib_str_suffixof s t = smtlib_str_contains t s"
-   by (simp add: smtlib_str_contains2_def smtlib_str_contains_equal smtlib_str_len_def smtlib_str_suffixof_def str_suffixof_one_lemma)
+  by (simp add: smtlib_str_contains2_def smtlib_str_contains_equal smtlib_str_len_def smtlib_str_suffixof_def str_suffixof_one_lemma)
 
 named_theorems rewrite_str_substr_combine1 \<open>automatically_generated\<close>
 
-lemma [rewrite_str_substr_combine1]: (*TODO*)
+lemma [rewrite_str_substr_combine1]:
   fixes s::"char list" and n1::"int" and m1::"int" and n2::"int" and m2::"int"
-  shows "(0::int) \<le> n1 \<and>
+  shows "NO_MATCH cvc_a (undefined s n1 m1 n2 m2) \<Longrightarrow> (0::int) \<le> n1 \<and>
    (0::int) \<le> n2 \<and> (0::int) \<le> m2 - (m1 - n2) \<longrightarrow>
    smtlib_str_substr (smtlib_str_substr s n1 m1) n2 m2 =
    smtlib_str_substr s (n1 + n2) (m1 - n2)"
-  unfolding smtlib_str_substr_def[of s n1 m1]
+unfolding smtlib_str_substr_def[of s n1 m1]
   apply (cases "n1 < int (length s)")
    apply simp_all
    apply (cases "0 < m1 ")
@@ -399,11 +465,12 @@ lemma [rewrite_str_substr_combine1]: (*TODO*)
     by (simp add: int_ops(6) of_nat_min smtlib_str_substr_def)
 
 
+
 named_theorems rewrite_str_substr_combine2 \<open>automatically_generated\<close>
 
-lemma [rewrite_str_substr_combine2]: (*TODO*)
+lemma [rewrite_str_substr_combine2]:
   fixes s::"char list" and n1::"int" and m1::"int" and n2::"int" and m2::"int"
-  shows "(0::int) \<le> n1 \<and>
+  shows "NO_MATCH cvc_a (undefined s n1 m1 n2 m2) \<Longrightarrow> (0::int) \<le> n1 \<and>
    (0::int) \<le> n2 \<and> (0::int) \<le> m1 - n2 - m2 \<longrightarrow>
    smtlib_str_substr (smtlib_str_substr s n1 m1) n2 m2 =
    smtlib_str_substr s (n1 + n2) m2"
@@ -432,10 +499,10 @@ named_theorems rewrite_str_substr_concat1 \<open>automatically_generated\<close>
 
 lemma [rewrite_str_substr_concat1]:
   fixes s1::"char list" and s2::"char list cvc_ListVar" and n::"int" and m::"int"
-  shows "(0::int) \<le> n \<and> n + m \<le> smtlib_str_len s1 \<longrightarrow>
+  shows "NO_MATCH cvc_a (undefined s1 s2 n m) \<Longrightarrow> (0::int) \<le> n \<and> n + m \<le> smtlib_str_len s1 \<longrightarrow>
    smtlib_str_substr (cvc_list_right smtlib_str_concat s1 s2) n m =
    smtlib_str_substr s1 n m"
-  apply (cases s2)
+   apply (cases s2)
   subgoal for s2s 
     apply (simp add: cvc_list_left_transfer cvc_list_right_transfer_op cvc_list_both_transfer_op)
     by (simp add: substr_concat1_lemma)
@@ -446,24 +513,24 @@ named_theorems rewrite_str_substr_full \<open>automatically_generated\<close>
 
 lemma [rewrite_str_substr_full]:
   fixes s::"char list" and n::"int"
-  shows "smtlib_str_len s \<le> n \<longrightarrow>
+  shows "NO_MATCH cvc_a (undefined s n) \<Longrightarrow> smtlib_str_len s \<le> n \<longrightarrow>
    smtlib_str_substr s (0::int) n = s"
-  unfolding smtlib_str_len_def smtlib_str_substr_def
-  using order_less_le by fastforce
+  apply (simp add: cvc_string_rewrite_defs)
+  using order_le_less by fastforce
 
 named_theorems rewrite_str_contains_refl \<open>automatically_generated\<close>
 
 lemma [rewrite_str_contains_refl]:
   fixes x::"char list"
-  shows "smtlib_str_contains x x = True"
-  by (metis append.right_neutral append_self_conv2 smtlib_str_contains2_def smtlib_str_contains_equal)
-
+  shows "NO_MATCH cvc_a (undefined x) \<Longrightarrow> smtlib_str_contains x x = True"
+  apply (simp add: cvc_string_rewrite_defs)
+  by (metis append.left_neutral append_Nil2)
 
 named_theorems rewrite_str_contains_concat_find \<open>automatically_generated\<close>
 
 lemma [rewrite_str_contains_concat_find]:
   fixes xs::"char list cvc_ListVar" and y::"char list" and zs::"char list cvc_ListVar"
-  shows "smtlib_str_contains
+  shows "NO_MATCH cvc_a (undefined xs y zs) \<Longrightarrow> smtlib_str_contains
     (cvc_list_right smtlib_str_concat (cvc_list_left smtlib_str_concat xs y)
       zs)
     y =
@@ -473,15 +540,22 @@ lemma [rewrite_str_contains_concat_find]:
   subgoal for zss xss 
     apply (simp add: cvc_list_left_transfer cvc_list_right_transfer_op cvc_list_both_transfer_op)
     apply (induction zss arbitrary: zs)
-    using str_eq_ctn_false_lemma apply blast
-    by (meson str_eq_ctn_false_lemma)
+    apply simp_all
+    apply (induction xss arbitrary: xs)
+    apply simp_all
+    apply (simp_all add: cvc_string_rewrite_defs)
+      apply (simp_all add: cvc_rewrites_fold)
+      apply (metis append.left_neutral append_Nil2)
+    apply (metis append.assoc)
+    by blast
   done
+
 
 named_theorems rewrite_str_contains_split_char \<open>automatically_generated\<close>
 
 lemma [rewrite_str_contains_split_char]:
   fixes x::"char list" and y::"char list" and z::"char list cvc_ListVar" and w::"char list"
-  shows "smtlib_str_len w = (1::int) \<longrightarrow>
+  shows "NO_MATCH cvc_a (undefined x y z w) \<Longrightarrow> smtlib_str_len w = (1::int) \<longrightarrow>
    smtlib_str_contains
     (cvc_list_right smtlib_str_concat (smtlib_str_concat x y) z) w =
    (smtlib_str_contains x w \<or>
@@ -492,22 +566,22 @@ lemma [rewrite_str_contains_split_char]:
     by (simp add: str_contains_split_char_lemma)
   done
 
+
 named_theorems rewrite_str_contains_leq_len_eq \<open>automatically_generated\<close>
 
 lemma [rewrite_str_contains_leq_len_eq]:
   fixes x::"char list" and y::"char list"
-  shows "smtlib_str_len x \<le> smtlib_str_len y \<longrightarrow>
+  shows "NO_MATCH cvc_a (undefined x y) \<Longrightarrow> smtlib_str_len x \<le> smtlib_str_len y \<longrightarrow>
    smtlib_str_contains x y = (x = y)"
   apply (induction x)
   using smtlib_str_contains2_def smtlib_str_contains_equal apply force
   using smtlib_str_contains_def smtlib_str_len_def by force
 
-
 named_theorems rewrite_str_concat_emp \<open>automatically_generated\<close>
 
 lemma [rewrite_str_concat_emp]:
   fixes xs::"char list cvc_ListVar" and ys::"char list cvc_ListVar"
-  shows "cvc_list_right smtlib_str_concat
+  shows "NO_MATCH cvc_a (undefined xs ys) \<Longrightarrow> cvc_list_right smtlib_str_concat
     (cvc_list_left smtlib_str_concat xs (''''::char list)) ys =
    cvc_list_both smtlib_str_concat [] xs ys"
   apply (cases ys)
@@ -517,32 +591,32 @@ lemma [rewrite_str_concat_emp]:
     by (simp add: str_concat_emp_lemma)
   done
 
+
 named_theorems rewrite_str_at_elim \<open>automatically_generated\<close>
 
 lemma [rewrite_str_at_elim]:
   fixes x::"char list" and n::"int"
-  shows "smtlib_str_at x n = smtlib_str_substr x n (1::int)"
-  by (simp add: smtlib_str_at_def)
+  shows "NO_MATCH cvc_a (undefined x n) \<Longrightarrow> smtlib_str_at x n = smtlib_str_substr x n (1::int)"
+    by (simp add: cvc_string_rewrite_defs)
 
 named_theorems rewrite_re_all_elim \<open>automatically_generated\<close>
 
 lemma [rewrite_re_all_elim]:
-  shows "smtlib_re_all = smtlib_re_star smtlib_re_allchar"
+  shows "NO_MATCH cvc_a (undefined ) \<Longrightarrow> smtlib_re_all = smtlib_re_star smtlib_re_allchar"
   by (simp add: smtlib_re_all_def)
 
 named_theorems rewrite_re_opt_elim \<open>automatically_generated\<close>
 
 lemma [rewrite_re_opt_elim]:
   fixes x::"char list set"
-  shows "\<forall>x::char list set.
-   smtlib_re_opt x = smtlib_re_union (smtlib_str_to_re (''''::char list)) x"
+  shows "NO_MATCH cvc_a (undefined x) \<Longrightarrow> smtlib_re_opt x = smtlib_re_union (smtlib_str_to_re (''''::char list)) x"
   using smtlib_re_opt_def smtlib_re_union_def by auto
 
 named_theorems rewrite_re_concat_emp \<open>automatically_generated\<close>
 
 lemma [rewrite_re_concat_emp]:
   fixes xs::"char list set cvc_ListVar" and ys::"char list set cvc_ListVar"
-  shows "cvc_list_right smtlib_re_concat
+  shows "NO_MATCH cvc_a (undefined xs ys) \<Longrightarrow> cvc_list_right smtlib_re_concat
     (cvc_list_left smtlib_re_concat xs (smtlib_str_to_re (''''::char list)))
     ys =
    cvc_list_both smtlib_re_concat ({''''}::char list set) xs ys"
@@ -553,12 +627,12 @@ lemma [rewrite_re_concat_emp]:
     by (simp add: re_concat_emp_lemma)
   done
 
+
 named_theorems rewrite_re_concat_none \<open>automatically_generated\<close>
 
 lemma [rewrite_re_concat_none]:
   fixes xs::"char list set cvc_ListVar" and ys::"char list set cvc_ListVar"
-  shows "\<forall>(xs::char list set cvc_ListVar) ys::char list set cvc_ListVar.
-   cvc_list_right smtlib_re_concat
+  shows "NO_MATCH cvc_a (undefined xs ys) \<Longrightarrow> cvc_list_right smtlib_re_concat
     (cvc_list_left smtlib_re_concat xs smtlib_re_none) ys =
    smtlib_re_none"
   apply (cases ys)
@@ -567,11 +641,12 @@ lemma [rewrite_re_concat_none]:
     by (metis cvc_ListVar.exhaust cvc_bin_op2.simps cvc_list_left_transfer cvc_list_right_def ex_in_conv smtlib_re_concat_foldr smtlib_re_concat_ind.cases smtlib_re_concat_smtlib_re_concat_induct smtlib_re_none_def)
   done
 
+
 named_theorems rewrite_re_concat_flatten \<open>automatically_generated\<close>
 
 lemma [rewrite_re_concat_flatten]:
   fixes xs::"char list set cvc_ListVar" and s::"char list set" and ys::"char list set cvc_ListVar" and zs::"char list set cvc_ListVar"
-  shows "cvc_list_right smtlib_re_concat
+  shows "NO_MATCH cvc_a (undefined xs s ys zs) \<Longrightarrow> cvc_list_right smtlib_re_concat
     (cvc_list_left smtlib_re_concat xs
       (cvc_list_right smtlib_re_concat s ys))
     zs =
@@ -587,11 +662,12 @@ lemma [rewrite_re_concat_flatten]:
     by (simp add: re_concat_flatten_lemma)
   done
 
+
 named_theorems rewrite_re_concat_star_swap \<open>automatically_generated\<close>
 
 lemma [rewrite_re_concat_star_swap]:
   fixes xs::"char list set cvc_ListVar" and r::"char list set" and ys::"char list set cvc_ListVar"
-  shows "cvc_list_right smtlib_re_concat
+  shows "NO_MATCH cvc_a (undefined xs r ys) \<Longrightarrow> cvc_list_right smtlib_re_concat
     (smtlib_re_concat (cvc_list_left smtlib_re_concat xs (smtlib_re_star r))
       r)
     ys =
@@ -606,12 +682,12 @@ lemma [rewrite_re_concat_star_swap]:
     by (simp add: re_concat_star_swap_lemma)
   done
 
+
 named_theorems rewrite_re_union_all \<open>automatically_generated\<close>
 
 lemma [rewrite_re_union_all]:
   fixes xs::"char list set cvc_ListVar" and ys::"char list set cvc_ListVar"
-  shows "
-   cvc_list_right smtlib_re_union
+  shows "NO_MATCH cvc_a (undefined xs ys) \<Longrightarrow> cvc_list_right smtlib_re_union
     (cvc_list_left smtlib_re_union xs (smtlib_re_star smtlib_re_allchar))
     ys =
    smtlib_re_star smtlib_re_allchar"
@@ -629,41 +705,17 @@ lemma [rewrite_re_union_all]:
     using smtlib_re_union_def by auto
   done
 
-named_theorems rewrite_re_union_none \<open>automatically_generated\<close>
-
-lemma [rewrite_re_union_none]:
-  fixes xs::"char list set cvc_ListVar" and ys::"char list set cvc_ListVar"
-  shows "cvc_list_right smtlib_re_union
-    (cvc_list_left smtlib_re_union xs smtlib_re_none) ys =
-   cvc_list_both smtlib_re_union ({}::char list set) xs ys"
-  apply (cases ys)
-  apply (cases xs)
-  subgoal for yss xss 
-    apply (simp add: cvc_list_left_transfer cvc_list_right_transfer_op cvc_list_both_transfer_op)
-    apply (induction yss arbitrary: ys)
-    apply simp_all
-        apply (induction xss arbitrary: xs)
-      apply simp_all
-    using cvc_ListOp_neutral_re_union smtlib_re_none_def apply force
-    using cvc_ListOp_neutral_re_union apply force
-    
-       apply (induction xss arbitrary: xs)
-     apply simp_all
-    using cvc_ListOp_neutral_re_union smtlib_re_none_def apply force
-    by (smt (verit, ccfv_threshold) Un_def foldr.simps(1) id_apply smtlib_re_none_def smtlib_re_union_def sup_aci(3) sup_bot.right_neutral)
-  done
-
 named_theorems rewrite_re_union_flatten \<open>automatically_generated\<close>
 
 lemma [rewrite_re_union_flatten]:
   fixes xs::"char list set cvc_ListVar" and b::"char list set" and ys::"char list set cvc_ListVar" and zs::"char list set cvc_ListVar"
-  shows "cvc_list_right smtlib_re_union
+  shows "NO_MATCH cvc_a (undefined xs b ys zs) \<Longrightarrow> cvc_list_right smtlib_re_union
     (cvc_list_left smtlib_re_union xs (cvc_list_right smtlib_re_union b ys))
     zs =
    cvc_list_right smtlib_re_union
     (cvc_list_right smtlib_re_union (cvc_list_left smtlib_re_union xs b) ys)
     zs"
-  apply (cases zs)
+ apply (cases zs)
   apply (cases ys)
   apply (cases xs)
   subgoal for zss yss xss 
@@ -701,7 +753,7 @@ named_theorems rewrite_re_union_dup \<open>automatically_generated\<close>
 
 lemma [rewrite_re_union_dup]:
   fixes xs::"char list set cvc_ListVar" and b::"char list set" and ys::"char list set cvc_ListVar" and zs::"char list set cvc_ListVar"
-  shows "cvc_list_right smtlib_re_union
+  shows "NO_MATCH cvc_a (undefined xs b ys zs) \<Longrightarrow> cvc_list_right smtlib_re_union
     (smtlib_re_union
       (cvc_list_right smtlib_re_union (cvc_list_left smtlib_re_union xs b)
         ys)
@@ -710,7 +762,7 @@ lemma [rewrite_re_union_dup]:
    cvc_list_right smtlib_re_union
     (cvc_list_right smtlib_re_union (cvc_list_left smtlib_re_union xs b) ys)
     zs"
-  apply (cases zs)
+ apply (cases zs)
   apply (cases ys)
   apply (cases xs)
   subgoal for zss yss xss 
@@ -727,9 +779,6 @@ lemma [rewrite_re_union_dup]:
     using smtlib_re_union_def by auto
   done
 
-
-named_theorems rewrite_re_inter_all \<open>automatically_generated\<close>
-
 lemma rewrite_re_inter_all_h1: "smtlib_re_inter (foldr smtlib_re_inter xss UNIV) A = foldr smtlib_re_inter xss A"
   apply (induction xss)
   apply (simp add: smtlib_re_inter_def)
@@ -737,13 +786,15 @@ lemma rewrite_re_inter_all_h1: "smtlib_re_inter (foldr smtlib_re_inter xss UNIV)
   by (smt (verit, ccfv_SIG) Collect_cong mem_Collect_eq smtlib_re_inter_def)
 
 
+named_theorems rewrite_re_inter_all \<open>automatically_generated\<close>
+
 lemma [rewrite_re_inter_all]:
   fixes xs::"char list set cvc_ListVar" and ys::"char list set cvc_ListVar"
-  shows "cvc_list_right smtlib_re_inter
+  shows "NO_MATCH cvc_a (undefined xs ys) \<Longrightarrow> cvc_list_right smtlib_re_inter
     (cvc_list_left smtlib_re_inter xs (smtlib_re_star smtlib_re_allchar))
     ys =
    cvc_list_both smtlib_re_inter (UNIV::char list set) xs ys"
-  apply (cases ys)
+ apply (cases ys)
   apply (cases xs)
   subgoal for yss xss 
     apply (simp add: cvc_list_left_transfer cvc_list_right_transfer_op cvc_list_both_transfer_op)
@@ -755,7 +806,7 @@ named_theorems rewrite_re_inter_none \<open>automatically_generated\<close>
 
 lemma [rewrite_re_inter_none]:
   fixes xs::"char list set cvc_ListVar" and ys::"char list set cvc_ListVar"
-  shows "cvc_list_right smtlib_re_inter
+  shows "NO_MATCH cvc_a (undefined xs ys) \<Longrightarrow> cvc_list_right smtlib_re_inter
     (cvc_list_left smtlib_re_inter xs smtlib_re_none) ys =
    smtlib_re_none"
   apply (cases ys)
@@ -771,6 +822,7 @@ lemma [rewrite_re_inter_none]:
     using smtlib_re_inter_def smtlib_re_none_def by auto
   done
 
+
 named_theorems rewrite_re_inter_flatten \<open>automatically_generated\<close>
 
 lemma rewrite_re_inter_flatten_h1: "smtlib_re_inter (foldr smtlib_re_inter xss (smtlib_re_inter b (foldr smtlib_re_inter yss UNIV))) A =
@@ -782,7 +834,7 @@ lemma rewrite_re_inter_flatten_h1: "smtlib_re_inter (foldr smtlib_re_inter xss (
 
 lemma [rewrite_re_inter_flatten]:
   fixes xs::"char list set cvc_ListVar" and b::"char list set" and ys::"char list set cvc_ListVar" and zs::"char list set cvc_ListVar"
-  shows "cvc_list_right smtlib_re_inter
+  shows "NO_MATCH cvc_a (undefined xs b ys zs) \<Longrightarrow> cvc_list_right smtlib_re_inter
     (cvc_list_left smtlib_re_inter xs (cvc_list_right smtlib_re_inter b ys))
     zs =
    cvc_list_right smtlib_re_inter
@@ -796,11 +848,12 @@ lemma [rewrite_re_inter_flatten]:
     by (simp add: rewrite_re_inter_flatten_h1)
   done
 
+
 named_theorems rewrite_re_inter_dup \<open>automatically_generated\<close>
 
 lemma [rewrite_re_inter_dup]:
   fixes xs::"char list set cvc_ListVar" and b::"char list set" and ys::"char list set cvc_ListVar" and zs::"char list set cvc_ListVar"
-  shows "cvc_list_right smtlib_re_inter
+  shows "NO_MATCH cvc_a (undefined xs b ys zs) \<Longrightarrow> cvc_list_right smtlib_re_inter
     (smtlib_re_inter
       (cvc_list_right smtlib_re_inter (cvc_list_left smtlib_re_inter xs b)
         ys)
@@ -827,23 +880,21 @@ lemma [rewrite_re_inter_dup]:
   done
 
 
-
 named_theorems rewrite_str_len_concat_rec \<open>automatically_generated\<close>
 
 lemma [rewrite_str_len_concat_rec]:
   fixes s1::"char list" and s2::"char list" and s3::"char list cvc_ListVar"
-  shows "smtlib_str_len
+  shows "NO_MATCH cvc_a (undefined s1 s2 s3) \<Longrightarrow> smtlib_str_len
     (cvc_list_right smtlib_str_concat (smtlib_str_concat s1 s2) s3) =
    smtlib_str_len s1 +
    smtlib_str_len (cvc_list_right smtlib_str_concat s2 s3)"
   apply (cases s3)
   subgoal for s3s 
-    apply (simp add: cvc_list_left_transfer cvc_list_right_transfer_op cvc_list_both_transfer_op)
-    by (simp add: str_len_concat_rec_lemma)
+    by (simp add: cvc_list_left_transfer cvc_list_right_transfer_op cvc_list_both_transfer_op)
   done
 
-named_theorems rewrite_str_in_re_range_elim \<open>automatically_generated\<close>
 
+named_theorems rewrite_str_in_re_range_elim \<open>automatically_generated\<close>
 
 lemma h1: "(of_char c1::int) \<ge> -1"
   unfolding of_char_def by simp
@@ -879,9 +930,5 @@ lemma [rewrite_str_in_re_range_elim]:
     using String_Rewrites.h2 linorder_not_le apply blast
     using String_Rewrites.h2 linorder_not_le by blast
   by (smt (verit, ccfv_SIG) String_Rewrites.h2 Suc_length_conv char_of_char length_greater_0_conv list.size(3) nth_Cons_0 string_comp.simps(3))
-
-declare[[show_types]]
-declare[[show_sorts]]
-
 
 end
