src/HOL/CVC/cvc5_dsl_rewrites/UF_Rewrites.thy
@@ -1,23 +1,32 @@
 theory UF_Rewrites
-  imports Dsl_Nary_Ops
+  imports "HOL-CVC.Dsl_Nary_Ops" 
 begin
 
-named_theorems rewrite_eq_symm \<open>added by hand\<close>
+(* Thank you for using IsaRARE. This is a theory automatically created from a RARE file!
+All that remains to do is to prove any lemma whose provided proof fails.
+If you want to use the lemmas for proof reconstruction you'll also need to import this file in Rare_Interface.thy*)
 
-lemma [rewrite_eq_symm]:
-  shows "NO_MATCH c (undefined a b) ==> a = b \<longleftrightarrow> b = a"
-  by auto
-
-named_theorems rewrite_eq_refl \<open>added by hand\<close>
+named_theorems rewrite_eq_refl \<open>automatically_generated\<close>
 
 lemma [rewrite_eq_refl]:
-  shows "NO_MATCH c (undefined a) ==> (a = a) = True"
+  fixes t::"'a::type"
+  shows "NO_MATCH cvc_a (undefined t) \<Longrightarrow> (t = t) = True"
   by auto
 
-named_theorems rewrite_distinct_binary_elim \<open>added by hand\<close>
+
+named_theorems rewrite_eq_symm \<open>automatically_generated\<close>
+
+lemma [rewrite_eq_symm]:
+  fixes t::"'a::type" and s::"'a::type"
+  shows "NO_MATCH cvc_a (undefined t s) \<Longrightarrow> (t = s) = (s = t)"
+  by auto
+
+
+named_theorems rewrite_distinct_binary_elim \<open>automatically_generated\<close>
 
 lemma [rewrite_distinct_binary_elim]:
-  shows "NO_MATCH c (undefined t s) ==> \<not>(t = s) = (\<not>(t = s))"
+  fixes t::"'a::type" and s::"'a::type"
+  shows "NO_MATCH cvc_a (undefined t s) \<Longrightarrow> (t \<noteq> s) = (t \<noteq> s)"
   by auto
 
 end
